unused params, some formatting

Cslib/Languages/LambdaCalculus/LocallyNameless/Untyped/MultiSubst.lean
@@ -33,58 +33,54 @@ abbrev Env (Var : Type u) := Context Var (Term Var)
 /-- Multi-substitution substitutes all target variables
     in an environment by their corresponding terms -/
 @[scoped grind =]
-def multiSubst (σ : Env Var) (M : Term Var) : Term Var :=
-  match σ with
+def multiSubst (E : Env Var) (M : Term Var) : Term Var :=
+  match E with
   | [] => M
-  | ⟨ i, sub ⟩ :: σ' => (multiSubst σ' M) [ i := sub ]
+  | ⟨i, sub⟩ :: E' => (multiSubst E' M) [ i := sub ]
 
 /-- The free variables of an environment are the union of
     the free variables of all terms in the environment.
     The target variables are not necessarily included -/
-@[scoped grind =]
 def Env.fv (E : Env Var) : Finset Var :=
   match E with
   | [] => {}
   | ⟨ _, sub ⟩ :: E' => sub.fv ∪ Env.fv E'
 
-/-- An environment is locally closed if all terms in the environment are locally closed -/
-abbrev env_LC (E : Env Var) : Prop := ∀ {x M}, ⟨ x, M ⟩ ∈ E → LC M
+attribute [scoped grind =] Env.fv
 
-omit [DecidableEq Var] in
+/-- An environment is locally closed if all terms in the environment are locally closed -/
+abbrev env_LC (E : Env Var) : Prop := ∀ {x M}, ⟨x, M⟩ ∈ E → LC M
+
 /-- Adding a locally closed term to an environment preserves local closure -/
-lemma env_LC_cons {E : Env Var} {x : Var} {sub : Term Var}
-  (lc_sub : LC sub) (lc_E : env_LC E)
-  : env_LC (⟨ x, sub ⟩ :: E) := by
-  intro y M h_mem
-  cases h_mem <;> aesop
+lemma env_LC_cons (lc_sub : LC sub) (lc_E : env_LC E) : env_LC (⟨ x, sub ⟩ :: E) := by
+  grind
 
 /-- Multi-substitution of a fresh variable does nothing -/
-lemma multiSubst_fvar_fresh (E : Env Var) :
-    ∀ x ∉ E.dom, multiSubst E (Term.fvar x) = Term.fvar x := by
-  induction E with grind [multiSubst]
+lemma multiSubst_fvar_fresh (E : Env Var) : ∀ x ∉ E.dom, multiSubst E (fvar x) = fvar x := by
+  induction E with grind
 
 /-- If x is neither a free variable of an environment Ns or a term M, then
     x is also not a free variable of the multi-substitution of Ns into M -/
 lemma multiSubst_preserves_not_fvar (M : Term Var) (E : Env Var) (nmem : x ∉ M.fv ∪ E.fv) :
     x ∉ (multiSubst E M).fv := by
-  induction E with grind [multiSubst, subst_preserve_not_fvar, Env.fv]
+  induction E with grind [subst_preserve_not_fvar]
 
 /-- Multi-substitution propagates recursively through an application -/
 lemma multiSubst_app (M N : Term Var) (E : Env Var) :
-      multiSubst E (Term.app M N) = Term.app (multiSubst E M) (multiSubst E N) := by
-  induction E with grind [multiSubst]
+    multiSubst E (app M N) = app (multiSubst E M) (multiSubst E N) := by
+  induction E with grind
 
 /-- Multi-substitution propagates recursively through an abstraction -/
 lemma multiSubst_abs (M : Term Var) (E : Env Var) :
-      multiSubst E (Term.abs M) = Term.abs (multiSubst E M) := by
-  induction E with grind [multiSubst]
+    multiSubst E (abs M) = abs (multiSubst E M) := by
+  induction E with grind
 
 /-- Multi-substitution commutes with opening a term with a fresh variable,
     provided that the variable is not in the domain of the environment
     and the environment is locally closed -/
 lemma multiSubst_open_var [HasFresh Var] (M : Term Var) (E : Env Var) (x : Var)
   (h_ndom : x ∉ E.dom) (h_lc : env_LC E) :
-    multiSubst E (M ^ Term.fvar x) = multiSubst E M ^ Term.fvar x := by
+    multiSubst E (M ^ fvar x) = multiSubst E M ^ fvar x := by
   induction E with grind
 
 end LambdaCalculus.LocallyNameless.Untyped.Term
